Let's analyze the given **recursive algorithm** and determine the **time complexity** and the value of \( T(6) \) for the function `function(int n)`.

### **Code Analysis**
```c
int function(int n)
{
    int i = 0;
    if (n <= 0)
    {
        return 0;
    }
    else
    {
        i = random(n - 1);    // Random call takes O(1) time
        printf("this\n");      // Print statement takes O(1) time
        return function(i) + function(n - 1 - i); // Recursive calls
    }
}
```

### **Step-by-Step Analysis**

#### **1. Base Case:**
```c
if (n <= 0)
{
    return 0;
}
```
- When \( n \leq 0 \), the function returns 0 immediately, which is a constant-time operation: \( O(1) \).

#### **2. Recursive Case:**
```c
i = random(n - 1);    // Random call takes O(1)
printf("this\n");      // Print statement takes O(1)
return function(i) + function(n - 1 - i); // Recursive calls
```
- The `random(n - 1)` call takes constant time, \( O(1) \).
- The `printf("this\n")` statement also takes constant time, \( O(1) \).
- The function then calls itself recursively twice: `function(i)` and `function(n - 1 - i)`.

#### **3. Recurrence Relation:**
- The function makes **two recursive calls**: one with \( i \) and one with \( n - 1 - i \), where \( i \) is a random integer between 0 and \( n - 1 \).
- The total time complexity \( T(n) \) for the function can be expressed as:
  \[
  T(n) = T(i) + T(n - 1 - i) + O(1)
  \]
  - The \( O(1) \) term accounts for the random number generation and the print statement.

---

### **Expected Time Complexity**
- The value of \( i \) is chosen randomly between 0 and \( n - 1 \), so on average, \( i \) will be around \( \frac{n}{2} \).
- Therefore, the recursive calls will split the problem roughly in half on average. This results in a **divide-and-conquer** recurrence relation, which resembles the **binary recursion** pattern.

- The recurrence relation is similar to:
  \[
  T(n) = 2T\left(\frac{n}{2}\right) + O(1)
  \]
  This is a typical recurrence for **binary recursion**, and by solving it (using the master theorem or recursion tree method), we get:
  \[
  T(n) = O(n)
  \]

---

### **Calculating \( T(6) \)**
To find \( T(6) \), we need to understand how the recursion unfolds. We can write out the recursive calls:

1. \( T(6) = T(i) + T(6 - 1 - i) + O(1) \)
2. \( i \) is randomly chosen between 0 and 5. Letâ€™s assume an average value of \( i = 2 \) (this is an approximation since \( i \) is random).
3. The function then becomes:
   \[
   T(6) = T(2) + T(3) + O(1)
   \]

Now, we recursively calculate \( T(2) \) and \( T(3) \):

- \( T(2) = T(i) + T(2 - 1 - i) + O(1) \), with \( i = 1 \) (on average):
  \[
  T(2) = T(1) + T(0) + O(1)
  \]
  - \( T(1) = T(0) + O(1) \)
  - \( T(0) = O(1) \)
  - So, \( T(2) = O(1) + O(1) + O(1) = O(1) \)

- \( T(3) = T(i) + T(3 - 1 - i) + O(1) \), with \( i = 1 \) (on average):
  \[
  T(3) = T(1) + T(2) + O(1)
  \]
  - \( T(1) = O(1) \)
  - \( T(2) = O(1) \)
  - So, \( T(3) = O(1) + O(1) + O(1) = O(1) \)

Thus, combining all the results:
\[
T(6) = T(2) + T(3) + O(1) = O(1) + O(1) + O(1) = O(1)
\]

---

### **Final Answer**
The value of \( T(6) \) is \( O(1) \), meaning that the **average time complexity** of the function for \( n = 6 \) is constant for each individual call.

